\documentclass[11pt, oneside]{article} 
\usepackage{geometry}
\geometry{letterpaper} 
\usepackage{graphicx}
	
\usepackage{amssymb}
\usepackage{amsmath}
\usepackage{parskip}
\usepackage{color}
\usepackage{hyperref}

\graphicspath{{/Users/telliott_admin/Tex/png/}}
% \begin{center} \includegraphics [scale=0.4] {gauss3.png} \end{center}

%break
\title{Parametrization}
\date{}

\begin{document}
\maketitle
\Large

\subsection*{General approach to parametrization and the Jacobian}
Suppose we wish to determine an area by integration and we're working with the unit square $x=0 \to x=1$ and $y=0 \to y=1$, sometimes written as $[\ 0,1\ ] \times [\ 0,1\ ]$.  The area is clearly just $1$.  Now we want to make a change of variables for some reason, maybe to work on a function that's easier to deal with after the substitution, or because we have some weird bounds in our problem.
\[ u = 3x-2y \]
\[ v = x + y \]
We figure out the "exchange rate" for area by tracing out the parallelogram formed by this linear transformation

\begin{align*}
& (0,0) \to (0,0) \\
& (1,0) \to (3,1) \\
& (0,1) \to (-2,1)
\end{align*}

If we think of the vectors from $0,0$ to $(3,1)$ as $\langle 3, 1 \rangle$,  and from $0,0$ to $(-2,1)$ as $\langle -2 ,1 \rangle$, the area of the parallelogram formed by these vectors is given by the determinant
\[
| \langle 3, 1 \rangle \times \langle -2 ,1 \rangle | =
\begin{vmatrix}
3 & -2 \\
1 & \ \ 1 
\end{vmatrix} = 5
\]
The other way to do this calculation is (as we've been doing)
\[ u_x = 3 \]
\[ u_y = -2 \]
\[ v_x = 1 \]
\[ v_y = 1 \]
The Jacobian
\[ J = 
\begin{vmatrix}
u_x & u_y \\
v_x & v_y 
\end{vmatrix} = 
\begin{vmatrix}
3 & -2 \\
1 & \ \ 1 
\end{vmatrix}
= 3 - (-2) = 5 \]
Or more simply
\[ J = u_x v_y - u_y v_x = 3  - (-2) = 5 \]
And again, since we took the derivatives with respect to $x$ and $y$, we multiply $dx \ dy$ by $J$.

Each element of the area determined in $uv$ units is worth $5$ of an element in $xy$ units.
\[ 5 \iint\limits_{R}  f(x,y) \ dx \ dy = \iint\limits_{R}  f(u,v) \ du \ dv \]
\begin{equation}
\boxed{du \ dv = J \ dx \ dy }
\end{equation}

To say the above one more time in slightly different language, we have
\[ u = u(x,y) \]
\[ v = v(x,y) \]
If we change $x$ by a little bit $\Delta x$ and $y$ by a little bit $\Delta y$, by how much do $u$ and $v$ change? 
The linear approximation is
\[ \Delta u = u_x \Delta x + u_y \Delta y \]
\[ \Delta v = v_x \Delta x + v_y \Delta y \]
So for $\Delta x = 1$, the vector $<1,0>$ becomes
\[ \ <u_x ,v_x> \]
and $<0,1>$ becomes
\[ \ <u_y ,v_y> \]
and the area of the parallelogram formed by these two vectors (the area in $uv$-coordinates) is the absolute value of the cross product (think of them as lying in the plane, so there is only one term)
\[ <u_x ,v_x> \ \times  <u_y ,v_y > \]
\[ J = u_x v_y - u_y v_x \]
So for each unit $dx \ dy$ we get $du \ dv = J \ dx \ dy $ in the $uv$-coordinate system.

\subsection*{Tilted ellipse}
Here is the equation of an ellipse, although that may be hard to recognize at first.
\[ x^2 + 4xy + 13y^2 = 16 \]
If you remember (or look up) the formula
\[ Ax^2 + Bxy + Cy^2 + Dx + Ey + F = 0 \]
\[ A,B,C = 1,4,13 \]
The discriminant is
\[ B^2 - 4AC = 16 - 52 = -36 < 0 \]
Since it's $ < 0 $, this is an ellipse.  Or we could just get a plotting program like Grapher to plot it
\begin{center} \includegraphics [scale=0.4] {tilted_ellipse.png} \end{center}

If we knew the angle of the tilt, and there is a method for that, we could rotate to a new coordinate system and just compute the area as $\pi ab$.  However, there is another way which I think is easier.  We "complete the square" to remove the term $4xy$ which "mixes" $x$ and $y$.  Since
\[ (x + 2y)^2 = x^2 + 4xy + 4y^2 \]
Our equation is transformed as follows
\[ x^2 + 4xy + 13y^2 = 16 \]
\[ \ [ \ x^2 + 4xy + 4y^2  \ ] \ + 9y^2  = 16 \]
\[ (x + 2y)^2 + 9y^2 = 16 \]
We do a substitution almost like before, but modified:
\[ u = x + 2y \]
\[ v = 3y \]
so now we have
\[ u^2 + v^2 = 16 \]
This is a circle of radius $4$ and area $16\pi$.
Now we just need the Jacobian:
\[ u_x = 1 \]
\[ u_y = 2 \]
\[ v_x = 0 \]
\[ v_y = 3 \]
\[ J = 
\begin{vmatrix}
u_x & u_y \\
v_x & v_y 
\end{vmatrix} = 
\begin{vmatrix}
1 & 2 \\
0 & 3 
\end{vmatrix}
= 3 \]
\[ du \ dv = 3 \ dx \ dy \]
When we took the partial derivatives, they were partials of $u,v$ with respect to $x,y$, so we end up multiplying $dx \ dy$ by J.
\[ \frac{1}{3} du \ dv = dx \ dy \]
We need to multiply the area by this factor to give a final answer of $16\pi/3$.

\subsection*{Varberg example}
The next example is from Varberg, 17.16.
\begin{center} \includegraphics [scale=0.6] {Varberg-17-16.png} \end{center}
We have the lines $x=y$ and $x=2y$ and the curves $xy=1$ and $xy=5$.  Looks like $xy$ would be a good variable to have so
\[ u = \frac{x}{y} \]
\[ v = xy \]
These suggestions come from Varberg, not me.  :)  

The boundaries of the region are just $u = 1 \rightarrow u = 2$ and $v = 1 \rightarrow v = 5 $.
Rearranging:
\[ x = uy \]
\[ x = \frac{v}{y} \]
\[ x^2 = xx = uy \ \frac{v}{y} =  uv \]

For the Jacobian, it is important to solve for $x,y$ in terms of $u,v$, and not the other way around, so that we'll have terms containing $u$ and $v$ in the final integral.
\[ x = \sqrt{uv} \]
\[ y^2 = \frac{x}{u} \frac{v}{x} = \frac{v}{u} \]
\[ y = \sqrt{\frac{v}{u}} \]
So 
\[ x_u = \frac{1}{2} \sqrt{\frac{v}{u}} \]
\[ x_v =  \frac{1}{2} \sqrt{\frac{u}{v}} \]
\[ y_u =  -\frac{1}{2u} \sqrt{\frac{v}{u}}\]
\[ y_v = \frac{1}{2} \sqrt{\frac{1}{uv}} \]
The Jacobian is then
\[ x_u y_v - x_v y_u \]
\[ \frac{1}{2} \sqrt{\frac{v}{u}} \ \frac{1}{2} \sqrt{\frac{1}{uv}} + \frac{1}{2} \sqrt{\frac{u}{v}} \  \frac{1}{2u} \sqrt{\frac{v}{u}} \]
\[ = \frac{1}{4u} + \frac{1}{4u} = \frac{1}{2u} \]
The area is 
\[ A = \iint\limits_{R} 1 \ dx \ dy =  \iint\limits_{R} \frac{1}{2u}  \ du \ dv \]
\[ = \int_{u=1}^{2} \ \int_{v=1}^{5} \frac{1}{2u}  \ dv \ du \]
\[ = 2 \int_{u=1}^{2} \ \frac{1}{u} \ du = 2 \ln 2 \]

\subsection*{spherical coordinates}
In a previous chapter, we found the volume element for the sphere as
\[ dV = \rho^2 \sin \phi \ d \rho \ d \phi \ d \theta \]
by analyzing the sides of the volume element.  We can do this more formally, using the Jacobian.  It is a bit of a mess but we get there in the end.

In 2D we write
\[ x = r \cos \theta \]
\[ y = r \sin \theta \]

In 3D we write
\[ x = \rho \sin \phi \cos \theta \]
\[ y = \rho \sin \phi \sin \theta \]
\[ z = \rho \cos \phi \]
\begin{center} \includegraphics [scale=0.4] {spherical_coordinates2.png} \end{center}

We need to compute $9$ partial derivatives:
\[ x_{\rho} = \sin \phi \cos \theta \]
\[ x_{\phi}  = \rho \cos \phi \cos \theta \]
\[ x_{\theta} = -\rho \sin \phi \sin \theta \]

\[ y_{\rho} = \sin \phi \sin \theta \]
\[ y_{\phi}  = \rho \cos \phi \sin \theta \]
\[ y_{\theta} = \rho \sin \phi \cos \theta \]

\[ z_{\rho} = \cos \phi \]
\[ z_{\phi}  = -\rho \sin \phi \]
\[ z_{\theta} = 0 \]

Compute the determinant of this $3 \times 3$ matrix:
\[ \begin{vmatrix}
x_{\rho} = \sin \phi \cos \theta && x_{\phi}  = \rho \cos \phi \cos \theta &&x_{\theta} = -\rho \sin \phi \sin \theta  \\
y_{\rho} = \sin \phi \sin \theta && y_{\phi}  = \rho \cos \phi \sin \theta && y_{\theta} = \rho \sin \phi \cos \theta  \\
z_{\rho} = \cos \phi &&  z_{\phi}  = -\rho \sin \phi && z_{\theta} = 0
\end{vmatrix} \]

We should use the third row or the third column because $z_{\theta} = 0$.  

We choose the third row because we notice that
\[ x_{\phi} y_{\theta} = \rho \cos \phi \cos \theta \ \rho \sin \phi \cos \theta = \rho^2 \sin \phi \cos \phi \cos^2 \theta \]
\[ x_{\theta} y_{\phi} = -\rho \sin \phi \sin \theta \ \rho \cos \phi \sin \theta = -\rho^2 \sin \phi \cos \phi \sin^2 \theta \]
So subtracting, we get 
\[ \rho^2 \sin \phi \cos \phi (\cos^2 \theta + \sin^2 \theta) \]
\[ = \rho^2 \sin \phi \cos \phi \]
Multiplying by $z_\rho$ gives
\[ = \rho^2 \sin \phi \cos^2 \phi \]
which should look vaguely familiar.

For the second term of the determinant we compute
\[ x_{\rho} y_{\theta} = \sin \phi \cos \theta \ \rho \sin \phi \cos \theta  = \rho \sin^2 \phi \cos^2 \theta \]
\[ x_{\theta} y_{\rho} = -\rho \sin \phi \sin \theta \ \sin \phi \sin \theta = -\rho \sin^2 \phi \sin^2 \theta \]
So, subtracting, we get
\[ = \rho \sin^2 \phi (\cos^2 \theta + \sin^2 \theta) \]
\[ = \rho \sin^2 \phi \]
Multiplying by $z_\phi$ gives
\[ - \rho^2 \sin^3 \phi \]

Finally, subtract the second term from the first:
\[ \rho^2 \sin \phi \cos^2 \phi + \rho^2 \sin^3 \phi  = \rho^2 \sin \phi \]
Which is exactly what we said before!



\end{document}