\documentclass[11pt, oneside]{article}   	% use "amsart" instead of "article" for AMSLaTeX format
\usepackage{geometry}                		% See geometry.pdf to learn the layout options. There are lots.
\geometry{letterpaper}                   		% ... or a4paper or a5paper or ... 
%\geometry{landscape}                		% Activate for for rotated page geometry
%\usepackage[parfill]{parskip}    		% Activate to begin paragraphs with an empty line rather than an indent
\usepackage{graphicx}				% Use pdf, png, jpg, or eps§ with pdflatex; use eps in DVI mode
								% TeX will automatically convert eps --> pdf in pdflatex		
\usepackage{amssymb}
\usepackage{amsmath}
\usepackage{parskip}

\title{The cycloid}
%\author{The Author}
\date{}							% Activate to display a given date or no date

\graphicspath{{/Users/telliott_admin/Dropbox/Tex/png/}}

\begin{document}

\maketitle

\Large
\noindent

We imagine a bicycle with one tire marked at a particular point on the rim, say with fluorescent paint or a small light.  We start at time $t = 0$ with that point $P$ in contact with the $x$ axis at $(0,0)$.  Then we start rolling the bike.  As the tire rotates our fixed point $P$ on the rim traces a curve
\begin{center} \includegraphics [scale=0.6] {cycloid.png} \end{center}

\begin{center} \includegraphics [scale=0.5] {cycloid2.png} \end{center}
We want to find parametric equations $x(t)$, $y(t)$ that give the position of the point $P$ as a function of time.  The second diagram above shows the angle through which the wheel has turned as $\theta$, but we will use $t$ for $\theta$ here.  The $x$ displacement of the vertical straight down from the center of the tire is just $at$, where $a$ is the radius of the wheel, it is equal to the arc on the circumference of the wheel from the point which is currently in contact with the ground, up to $P$.

It is fairly easy to derive the desired parametric equations, using vectors.  For $x$, we have the vector that goes from $(0,0)$ to the contact point with the ground.  As indicated in the figure, that is $at$.  We need to subtract the distance $a \ sin\ t$ from that.  It's easier to see for $t < \pi/2$, but it is true always.  This is the usual circular motion, just with the circle flipped so the motion is clockwise, and we started at the bottom.

For $y$, we have a constant factor of $a$ above the $x$ axis, then the additional displacement is $-a \ cos \ t$.  So for $t=0$ we have the additional displacement is -a (we were on the ground), for $t=\pi/2$ it is zero, and for $t=\pi$ it is plus $a$ for a total of $2a$.

The parametric equations are then
\begin{align*} 
x(t) = at - a \ sin\ t \\
y(t) = a - a \ cos\ t \\
x'(t) = a - a \ cos\ t \\
y'(t) = a \ sin\ t  \\
\end{align*} 

The derivation above did a little mental gymnastics with the circle, flipping it and setting $t=0$ when the point is at the bottom.  As an alternative, leave the circle in its usual orientation, with an angle $s$ to the positive $x$ axis.

It can be seen easily that $s$ and $t$ are related by the equation 
\[ s = 3\pi/2 - t \]

The vector from the center of the circle to the point on the edge is just the standard one for a point on a circle of radius $a$:
\[ a \ \langle \cos s, \sin s  \rangle \]
For the $x$ component:
\[ \cos s = \cos 3 \pi / 2 - t \]
\[ = \cos 3 \pi / 2  \cos t + \sin 3 \pi / 2 \sin t \]
Recall that $\cos 3 \pi / 2 = 0$ and $\sin 3 \pi / 2 = -1$ so
\[ \cos s = - \sin t \]
And for the $y$ component
\[ \sin s = \sin 3 \pi / 2 - t \]
\[ = \sin 3 \pi / 2 \cos t - \sin t \cos  3 \pi / 2 \]
\[ = - \cos t \]
The vector is then
\[ a \ \langle \cos s, \sin s  \rangle = a \ \langle -\sin t, -\cos t  \rangle \]

In addition, we have to add another vector, one extending from the origin to the center of the wheel.  The $y$ component is constant, it is just $a$.  The $x$-component is the distance the wheel has traveled from its initial position (the distance between the origin and the point of contact with the $x$-axis, which is $at$, shown as $a \theta$ in the figure).

Hence the vector to the point is:
\[ a \ \langle -\sin t, -\cos t  \rangle + \langle at, a \rangle \]
\[ a \ \langle t - \sin t, 1 - \cos t \rangle \]

which matches what we had before.

\subsection*{Arc length}

We wish to determine the arc length and area under the curve for a complete revolution of the wheel.

We want to use a slightly different version of the usual formula for arc length

\[ ds^2 = dx^2 + dy^2 \]
\[ (\frac{ds}{dt})^2 = (\frac{dx}{dt})^2 + (\frac{dy}{dt})^2 \]
\[ ds = \sqrt{(\frac{dx}{dt})^2 + (\frac{dy}{dt})^2} \ dt = \sqrt{(a - a \cos\ t)^2 + (a \sin\ t)^2} \ dt  \]
This expands to
\[ a \sqrt{1 - 2 \cos\ t + \cos^2t + \sin^2t } \ dt =  a \sqrt{2 - 2 \cos \ t} \ dt\] 
The length is
\[ L = \int_0^{2\pi} a \sqrt{2 - 2 \cos \ t} \ dt\]
\[ = a \sqrt{2} \ \int_0^{2\pi} \sqrt{1 - \cos \ t} \ dt\]

\subsection*{double angle}

\[ \cos (s-t) = \cos s \cos t + \sin s \sin \ t \]
(check:  if $s=t$ then $\cos 0 = 1$, which is correct).

So
\[ \cos (s+t) = \cos s \cos t - \sin s \sin \ t \]
Let $s = t$ and $u = 2s$, then
\[ \cos 2s = \cos u = \cos^2 \ (\frac{u}{2}) - \sin^2 \ (\frac{u}{2}) \]
\[ \cos u = 1 - \sin^2 \ (\frac{u}{2}) - \sin^2 \ (\frac{u}{2}) \]
\[ 2 \sin^2 \ (\frac{u}{2}) = 1 - \cos u \]
$u$ is just a dummy variable, so we can switch back to $t$
\[ 2 \sin^2 \ (\frac{t}{2}) = 1 - \cos t \]

\subsection*{finishing up}
We have that 
\[ L = a \sqrt{2} \ \int_0^{2\pi} \sqrt{1 - \cos \ t} \ dt\]

\[ 1 - \cos t = 2 \sin^2(\frac{t}{2}) \]
\[ \sqrt{1 - \cos t} = \sqrt{2} \sin(\frac{t}{2}) \]
So
\[ L = a \sqrt{2} \ \int_0^{2\pi} \sqrt{2} \sin \ (\frac{t}{2}) \ dt\]
\[  2a  \ \int_0^{2\pi} \sin \ (\frac{t}{2}) \ dt\]
\[ = 2a \ (-2) \cos \ (\frac{t}{2})\ \bigg |_0^{2\pi} \]
\[ = -4a \ (\cos \ \pi - \cos \ 0) \]
\[ = -4a \ (-1 - 1) = 8a\]
A simple answer to the problem.

\subsection*{Area under the arc}
We want
\[ A = \int_{t=0}^{t=2\pi} y \ dx \]
\[ = \int_{t=0}^{t=2\pi} (a - a \cos\ t) (a - a \cos\ t) \ dt \]
\[ a^2\int_{t=0}^{t=2\pi} (1 - \cos\ t) (1 - \cos\ t) \ dt \]
\[ a^2\int_{t=0}^{t=2\pi} (1 - 2 \cos\ t + \cos^2\ t) \ dt \]
If you don't remember the result for $\int \cos^2 t \ dt$, you can go back to the double angle formula above and convert from $\sin^2$ to $\cos^2$.  Otherwise recall it and write:
\[ A = a^2 ( t - 2 \sin \ t + \frac{1}{2}t + \frac{1}{4} \sin 2t ) \ \bigg|_0^{2\pi} \]
\[ a^2 ( 2\pi - 0 + \pi + 0 - 0 + 0 - 0 - 0    ) = 3\pi a^2 \]
Also a very simple answer.

\end{document}  