\documentclass[11pt, oneside]{article} 
\usepackage{geometry}
\geometry{letterpaper} 
\usepackage{graphicx}
	
\usepackage{amssymb}
\usepackage{amsmath}
\usepackage{parskip}
\usepackage{color}
\usepackage{hyperref}

\graphicspath{{/Users/telliott_admin/Tex/png/}}
% \begin{center} \includegraphics [scale=0.4] {gauss3.png} \end{center}

\title{Differentiate}
\date{}

\begin{document}
\maketitle
\Large

This section contains a general discussion of differentiation of complex functions.  A complex function takes as input a complex number, and emits as output another complex number.  

More concretely, a complex function is really a pair of functions defined on the real numbers:

\[ f(z) = f(x + iy) = u(x,y) + i \cdot v(x,y) \]

$u$ and $v$ each take two real numbers and emit one real number.  The output of $v$ is multiplied by $i$.  Here is an example:
\[ z = x + iy \]
\[ z^2 = (x + iy)(x + iy) \]
\[ = x^2 - y^2 + 2ixy \]
So $u(x,y) = x^2 - y^2$ and $v(x,y) = 2xy$.

Another one is:
\[ \frac{1}{z} = \frac{z*}{zz*} \]
\[ = \frac{x - iy}{(x + iy)(x - iy)} \]
\[ = \frac{x}{x^2 + y^2} + i \frac{-y}{x^2 + y^2} \]

Often a simplified notation is employed:

\[ f(z) = u + i \cdot v \]

Since the inputs cover the entire complex plane, we cannot plot graphs as with real functions.  Instead, one version of the complex plane is mapped by the function into a different version of the complex plane.

This chapter gives us a first glimpse of the important Cauchy-Riemann conditions and justifies one of the formulas for calculating the derivative

\[ f'(z) = u_x + i v_x \]

As an example of its use, consider the complex exponential
\[ f(z) = e^z \]
If we write $z = x + iy$ then
\[ f(z) = e^{x + iy} \]
\[ = e^x e^{iy} \]
and (from Euler):
\[ e^{iy} = \cos y + i \sin y \]
so
\[ f(z) = e^x \cos y + i e^x \sin y \]

Using the formula, it can be shown easily that the derivative is the same as the function itself, just as for the case of real numbers.
\[ u(x,y) = e^x \cos y \]
\[ u_x = e^x \cos y = u \]
\[ v(x,y) = e^x \sin y \]
\[ v_x = e^x \sin y = v \]
Hence
\[f'(z) = u_x + iv_x = z \]

\subsection*{definition}
We define the derivative $f'(z)$ of a complex function $f(z)$ similarly to the derivative of a real function:
\[ f'(z) = \lim_{w \rightarrow z} \ \frac{f(w) - f(z)}{w-z} \]
if the limit exists.

Alternatively, with $\Delta$ notation, we might write:
\[ f'(z) = \lim_{\Delta z \rightarrow 0} \ \frac{f(z + \Delta z) - f(z)}{\Delta z} \]

A crucial difference from real functions is that there are only two directions from which to approach a given real number $x$, while there is an infinite number of ways of approaching $z$ in the Argand plane.  The limit is over \emph{all} possible ways of approaching $z$.  

If the limit exists, the function $f$ is called differentiable and $f'(z)$ is the derivative.
Consider
\[ f(z) = u(x,y) + i v(x,y) \]
Then
\[ f'(z) = \frac{f(z + \Delta z) - f(z)}{\Delta z} \]
\[ = \frac{u(x + \Delta x, y + \Delta y) + i v (x + \Delta x, y + \Delta y) - u(x,y) - i v(x,y)}{\Delta x + i \Delta y} \]

\subsection*{fixed y}
We tame this beast by looking at two specific paths.

Looking at the special path along the $x$-axis where $\Delta y = 0$ we obtain
\[ f'(z) = \frac{u(x + \Delta x, y) + i v (x + \Delta x, y) - u(x,y) - i v(x,y)}{\Delta x} \]
Rearrange the numerator
\[ = \frac{u(x + \Delta x, y) - u(x,y)}{\Delta x} + \frac{i v (x + \Delta x, y) - i v(x,y)}{\Delta x} \]
The first term is
\[ u_x = \frac{\partial u}{\partial x} \]
and the second term is 
\[ i v_x \]
Hence we conclude that
\[ f'(z) = u_x + i v_x \]

\subsection*{fixed x}
Now look at the special path along the $y$-axis where $\Delta x = 0$:
\[ f'(z) = \frac{u(x, y + \Delta y) + i v (x, y + \Delta y) - u(x,y) - i v(x,y)}{i \Delta y} \]
Rearrange the numerator
\[ = \frac{u(x, y + \Delta y) - u(x,y)}{i \Delta y} + \frac{i v (x, y + \Delta y) - i v(x,y)}{i \Delta y} \]
\[ = \frac{1}{i} u_y + v_y \]
Recall that $1/i = -i$
\[ f'(z) = v_y - i u_y \]

\subsection*{Putting it together}
We require that the limit be the same regardless of the direction of approach to $z$, so these two expressions for the difference quotient must be equal:
\[ f'(z) = u_x + i v_x = - i u_y + v_y \]

Both the real and the imaginary parts must be equal so
\[ u_x  = v_y \]
\[ u_y = - v_x \]

Once differentiability is established, we can use whichever path we want to evaluate the derivative.

As we said at the beginning, in looking at various complex functions we can use this fact:
\[ f'(z) = u_x + i v_x \]

One consequence is that
\[ \frac{df}{dz} = \frac{\partial f}{\partial x} \]
and since
\[ = u_x + i v_x = v_y - i v_x \]
\[ = - i v_x + v_y \]
\[ = -i (v_x + i v_y) \]
\[ = -i \frac{\partial f}{\partial y} \]

We conclude that 
\[ \frac{df}{dz} = -i \frac{\partial f}{\partial y} \]

\subsection*{more}
When we get to integration in a later section we will find that we integrate complex functions as line integrals along a specified curve (perhaps a circle centered either on the origin or on a point $z_0$).  This curve relates the values of $x$ and $y$ and allows us to parametrize either $y$ in terms of $x$ or more generally, both $x$ and $y$ in terms of a single real variable or parameter $t$.

When we have a function of such a variable like
\[ f(t) = u(t) + i v(t) \]
then the derivative is defined to be
\[ f'(t) = u'(t) + i v'(t) \]
where $u$ and $v$ are real-valued functions of a single real variable and so follow the standard rules from introductory calculus.  In particular if
\[ w(t) = z_0 f(t) \]
then
\[ w'(t) = z_0 f'(t) \]
We can show this by using a little algebra:
\[ \frac{d}{dt} \ z_0 f(t) = \ [ \ (x_0 + i y_0) (u + iv) \ ]' \]
\[ = \ [ \ (x_0 u - y_0 v) + i (y_0 u + x_0 v) \ ]' \]
\[ = (x_0 u - y_0 v)' + i (y_0 u + x_0 v)' \]
\[ = (x_0 u' - y_0 v') + i (y_0 u' + x_0 v') \]
\[ = (x_0 + i y_0)(u' + iv') \]
\[ = z_0 \frac{d}{dt} \ f(t) \]
Thus
\[ \frac{d}{dt} \ z_0 f(t) = z_0 \frac{d}{dt} \ f(t) \]

Another expected result is
\[ \frac{d}{dt} \ e^{z_0 t} = z_0 e^{z_0 t} \]
where $z_0$ is a complex constant and $t$ is a real variable.

To do this one, refer to the definition
\[ f'(t) = u'(t) + i v'(t) \]
and now we need to break up the exponential into its real and imaginary parts.  

We write as we did above
\[ e^z = e^{x + iy} \]
\[ = e^x \ e^{iy} \]
by Euler's equation
\[ = e^x \ (\cos y + i \sin y) \]
\[ = e^x \cos y + i e^x \sin y \]

For the exponential with a constant we have
\[ e^{z_0 t} = e^{(x_0 + iy_0) t} \]
\[ = e^{x_0t} \ e^{i y_0 t} \]
\[ = e^{x_0t} \ (\cos y_0 t + i \sin y_0 t) \]
\[ = e^{x_0t} \cos y_0 t + i e^{x_0t} \ \sin y_0 t \]

Using the definition above we get that the derivative is
\[ \frac{d}{dt} \ e^{z_0 t} = x_0 e^{x_0t} \cos y_0 t  - y_0 e^{x_0t} \sin y_0 t + i(x_0 e^{x_0t} \sin y_0 t + y_0 e^{x_0t} \cos y_0 t) \]
\[ = x_0(e^{x_0t} \cos y_0 t + i e^{x_0 t} \sin y_0 t) + i y_0(e^{x_0t} \cos y_0 t + i e^{x_0 t} \sin y_0 t) \]
\[ = x_0 e^{z_0 t} + i y_0 e^{z_0 t} \]
\[ = (x_0 + iy_0) e^{z_0 t} \]
\[ = z_0 e^{z_0 t} \]
$\square$


\end{document}  