\documentclass[11pt, oneside]{article} 
\usepackage{geometry}
\geometry{letterpaper} 
\usepackage{graphicx}
	
\usepackage{amssymb}
\usepackage{amsmath}
\usepackage{parskip}
\usepackage{color}
\usepackage{hyperref}

\graphicspath{{/Users/telliott_admin/Dropbox/Tex/png/}}
% \begin{center} \includegraphics [scale=0.4] {gauss3.png} \end{center}

\title{Summary}
\date{}

\begin{document}
\maketitle
\Large

\subsection*{unit vectors and velocity}
The position vector (from the sun to the planet) is $\mathbf{r}$.  Starting from our definition of the unit vector in the $\mathbf{r}$ direction as
\[ \mathbf{u_r} = \ \langle \cos \theta, \sin \theta \rangle \]
where $\theta$ is the angle with the positive $x$-axis, we find $\mathbf{u_{\theta}} \perp \mathbf{u_r}$
\[ \mathbf{u_{\theta}} = \ \langle -\sin \theta, \cos \theta \rangle \]
and confirm orthognality
\[ \mathbf{u_r} \cdot \mathbf{u_{\theta}} = 0 \]
Remembering that $\theta = \theta(t)$, we easily obtain by the chain rule
\[ \dot{\mathbf{u}}_\mathbf{r} = \dot{\theta} \mathbf{u_{\theta}} \]
\[  \dot{\mathbf{u}}_\mathbf{\theta} = -\dot{\theta} \mathbf{u_{r}} \]
$r$ is the magnitude of $\mathbf{r}$
\[ \mathbf{r} = r \mathbf{u_r} \]
The velocity $\mathbf{v}$
\[ \mathbf{v} = \dot{\mathbf{r}} = \dot{r} \mathbf{u_r} + r \dot{\mathbf{u}}_\mathbf{r}  =  \dot{r} \mathbf{u_r} +  r \dot{\theta}  \mathbf{u_{\theta}}\]
We use a vector identity that is easy to prove
\[ \frac{d}{dt} \ (\mathbf{a} \times \mathbf{b}) = \dot{\mathbf{a}} \times \mathbf{b} + \mathbf{a} \times \dot{\mathbf{b}} \]
to calculate with Feynman's "dots"
\[ \frac{d}{dt} \ (\mathbf{r} \times \mathbf{v}) \]
\[ =  \frac{d}{dt} \ (\mathbf{r} \times \dot{\mathbf{r}}) \]
\[  =  \dot{\mathbf{r}} \times \dot{\mathbf{r}} +  \mathbf{r} \times \ddot{\mathbf{r}} = 0\]
because any vector's cross-product with itself is zero (including minus itself), which is true for the second term involving the acceleration.
\subsection*{acceleration}
An actual expression for the acceleration is just a matter of working through the dots
\[ \mathbf{a} = \dot{\mathbf{v}} = \ddot{\mathbf{r}} = \frac{d}{dt} \ (\dot{r}\mathbf{u_r} + r \dot{\theta} \mathbf{u_{\theta}}) \]
 \[ = \ddot{r}\mathbf{u_r} + \dot{r}\dot{\mathbf{u}}_\mathbf{r} + \dot{r} \dot{\theta} \mathbf{u_{\theta}} + r \ddot{\theta} \mathbf{u_{\theta}} + r \dot{\theta}  \dot{\mathbf{u}}_\mathbf{\theta}\]
substituting for $\dot{\mathbf{u}}_\mathbf{r}$ and $\dot{\mathbf{u}}_\mathbf{\theta}$ from above
\[ = \ddot{r}\mathbf{u_r} + \dot{r}\dot{\theta} \mathbf{u_{\theta}} + \dot{r} \dot{\theta} \mathbf{u_{\theta}} + r \ddot{\theta} \mathbf{u_{\theta}} - r \dot{\theta}^2  \mathbf{u}_\mathbf{r}\]
\[ = (\ddot{r} - r \dot{\theta}^2)  \mathbf{u}_\mathbf{r} + (2\dot{r} \dot{\theta} + r \ddot{\theta}) \mathbf{u_{\theta}}  \]
Rewrite the coefficient for $\mathbf{u_{\theta}}$ as
\[  \frac{1}{r}(2r \dot{r} \dot{\theta} + r^2\ddot{\theta}) = \frac{1}{r} \frac{d}{dt} (r^2\dot{\theta})  \]
\subsection*{angular momentum}
We find that the acceleration $\mathbf{a} = \dot{\mathbf{v}}$ has two parts of which the second (in $\mathbf{u_{\theta}}$)
\[ \frac{1}{r} \ \frac{d}{dt} \ r^2 \dot{\theta} = 0 \]
 is zero because $\mathbf{a}$ is all radial.  Hence $r^2 \dot{\theta} = h$ where $h$ is a constant.  Multiplied by the mass $m$, $mh$ becomes the conserved quantity, angular momentum.  It is also twice the area "swept out" and this is the statement of K2.

We get the vector $\mathbf{h}$ by defining the plane of motion as the $xy$-plane ($\mathbf{u_r} \times \mathbf{u_{\theta}} = \hat{\mathbf{k}}$) and
\[ \mathbf{h} = \mathbf{r} \times \mathbf{v} = r \mathbf{u_r} \times (\dot{r} \mathbf{u_r} +  r \dot{\theta}  \mathbf{u_{\theta}}) \]
the first term is zero so
\[ = r^2  \dot{\theta} ( \mathbf{u_r} \times \mathbf{u_{\theta}} ) = r^2  \dot{\theta}  \ \hat{\mathbf{k}} \]

\subsection*{key step}

With these preliminary steps we come to the key part of the derivation.  I like Varberg's version best.  The radial acceleration is
\[ \mathbf{a} = -\frac{GM}{r^2} \mathbf{u_r} \]
Compute $\mathbf{a} \times \hat{\mathbf{k}}$ (recall that $\mathbf{a}$ is in the $-\mathbf{u_r}$ direction) by recognizing that $-\mathbf{u_r} \times \hat{\mathbf{k}} = \mathbf{u_{\theta}}$ so
\[ \mathbf{a} \times \hat{\mathbf{k}} = \frac{GM}{r^2} \mathbf{u_{\theta}} \]
but from above $\dot{\mathbf{u}}_\mathbf{r} = \dot{\theta} \mathbf{u_{\theta}}$ so we have the crucial substitution:
\[ \mathbf{a} \times \hat{\mathbf{k}} = \frac{GM}{r^2 \dot{\theta} } \dot{\mathbf{u}}_\mathbf{r} \]
\[ \mathbf{a} \times \hat{\mathbf{k}} = \frac{GM}{h} \dot{\mathbf{u}}_\mathbf{r} \]
Now we just integrate with respect to time and get
\[ \int \mathbf{a} \times \hat{\mathbf{k}} = \int \frac{GM}{h} \dot{\mathbf{u}}_\mathbf{r}  \]
\[ \mathbf{v} \times \hat{\mathbf{k}} = \frac{GM}{h} \mathbf{u}_\mathbf{r} + \mathbf{d} \]
where $\mathbf{d}$ is a constant \emph{vector} of integration.
One last trick, we dot with $\mathbf{r}$ and simplify the left-hand side dramatically
\[ \mathbf{r} \cdot ( \mathbf{v} \times \hat{\mathbf{k}}) = (\mathbf{r} \times \mathbf{v}) \cdot  \hat{\mathbf{k}} = \mathbf{h} \cdot \hat{\mathbf{k}} = h \]
So
\[ h = \mathbf{r} \cdot (\frac{GM}{h} \mathbf{u}_\mathbf{r} + \mathbf{d}) \]
\[ \frac{h^2}{GM} = \mathbf{r} \cdot (\mathbf{u}_\mathbf{r} + \frac{h}{GM} \mathbf{d} ) \]
Define $k = h^2/GM$ and $e = hd/GM$ and $\theta$ as the angle between the constant vector $\mathbf{d}$ and $\mathbf{u}_\mathbf{r}$, so finally
\[ k = r (1 + e \cos \theta) \]
which for $e < 1$ is an ellipse.

\end{document}  